PrimitiveSize.v
@@ -1,0 +1,53 @@
+Require Import Termination.Trees.
+Require Import Termination.Syntax.
+Require Import Termination.Tactics.
+
+(* always 0 for non-values *)
+Fixpoint tsize_semantics t: nat :=
+  match t with
+  | fvar _ _ => 0
+  | lvar _ _ => 0
+  | err => 0
+
+  | uu => 0
+
+  | tsize t => 0
+
+  | notype_lambda t' => 0
+  | lambda T t' => 0
+  | app t1 t2 => 0
+
+  | pp t1 t2 => 1 + tsize_semantics t1 + tsize_semantics t2
+  | pi1 t' => 0
+  | pi2 t' => 0
+
+  | ttrue => 0
+  | tfalse => 0
+  | ite t1 t2 t3 => 0
+
+  | zero => 0
+  | succ t' =>  1 + tsize_semantics t'
+  | notype_rec t' t0 ts => 0
+  | rec T t' t0 ts => 0
+  | tmatch t' t0 ts => 0
+
+  | tfix T t' => 0
+  | notype_tfix t' => 0
+
+  | notype_tlet t1 t2 => 0
+  | tlet t1 A t2 => 0
+  | trefl => 0
+
+  | type_abs t => 0
+  | type_inst t T => 0
+  | notype_inst t => 0
+
+  | tfold t => 1 + tsize_semantics t
+  | tunfold t => 0
+
+  | tright t => 1 + tsize_semantics t
+  | tleft t => 1 + tsize_semantics t
+  | sum_match t tl tr => 0
+
+  | T => 0
+  end.
