ReducibilityPrimitiveSizeRules.v
@@ -1,0 +1,46 @@
+Require Import Equations.Equations.
+
+Require Import Termination.Tactics.
+Require Import Termination.Trees.
+Require Import Termination.Syntax.
+Require Import Termination.TermList.
+Require Import Termination.AssocList.
+Require Import Termination.StarRelation.
+Require Import Termination.SmallStep.
+Require Import Termination.PrimitiveSize.
+Require Import Termination.StarLemmas.
+
+Require Import Termination.ReducibilityDefinition.
+Require Import Termination.ReducibilityLemmas.
+Require Import Termination.ReducibilityCandidate.
+Require Import Termination.RedTactics.
+
+Opaque reducible_values.
+
+Lemma reducible_values_tsize:
+  forall theta n,
+    reducible_values theta (build_nat n) T_nat.
+Proof.
+  repeat step || simp_red;
+    eauto using is_nat_value_build_nat.
+Qed.
+
+Lemma reducible_tsize:
+  forall theta t T,
+    valid_interpretation theta ->
+    reducible theta t T ->
+    reducible theta (tsize t) T_nat.
+Proof.
+  unfold reducible, reduces_to; repeat step.
+  eexists (build_nat (tsize_semantics t')); steps; eauto using reducible_values_tsize;
+    eauto 6 using star_smallstep_trans, red_is_val with bsteplemmas smallstep.
+Qed.
+
+Lemma open_reducible_tsize:
+  forall tvars gamma t T,
+    open_reducible tvars gamma t T ->
+    open_reducible tvars gamma (tsize t) T_nat.
+Proof.
+  unfold open_reducible; steps;
+    eauto using reducible_tsize.
+Qed.
