WFLemmasEval.v
@@ -7,28 +7,6 @@ Require Import Termination.ListUtils.
 Require Import Termination.SizeLemmas.
 Require Import Termination.StarRelation.
 
-Lemma wf_smallstep:
-  forall t1 t2,
-    small_step t1 t2 ->
-    wf t1 0 ->
-    wf t2 0.
-Proof.
-  induction 1; steps; eauto with step_tactic bwf.
-Qed.
-
-Hint Resolve wf_smallstep: bwf.
-
-Lemma wf_star_smallstep:
-  forall t1 t2,
-    star small_step t1 t2 ->
-    wf t1 0 ->
-    wf t2 0.
-Proof.
-  induction 1; steps; eauto using wf_smallstep.
-Qed.
-
-Hint Resolve wf_star_smallstep: bwf.
-
 Lemma wf_nat_value:
   forall v, is_nat_value v -> wf v 0.
 Proof.
@@ -44,3 +22,25 @@ Proof.
 Qed.
 
 Hint Resolve twf_nat_value: btwf.
+
+Lemma wf_smallstep:
+  forall t1 t2,
+    small_step t1 t2 ->
+    wf t1 0 ->
+    wf t2 0.
+Proof.
+  induction 1; steps; eauto using is_nat_value_build_nat with step_tactic bwf.
+Qed.
+
+Hint Resolve wf_smallstep: bwf.
+
+Lemma wf_star_smallstep:
+  forall t1 t2,
+    star small_step t1 t2 ->
+    wf t1 0 ->
+    wf t2 0.
+Proof.
+  induction 1; steps; eauto using wf_smallstep.
+Qed.
+
+Hint Resolve wf_star_smallstep: bwf.
